theories/ExampleStack.v
@@ -1,3 +1,4 @@
+
 (**
 
 This file provides examples of the verification of a mutable stack,
